# The Master Theorem

---

# Motivation
- (Asymptotically) solves recurrence relationships
- Including:
  - Straightforward ones (from first year)
  - Harder ones (from this course)
- You need to:
  - **Know** the result
  - Be able to **apply** the result
- (You don't need to know the proof)

# Examples
## Binary Search
> ğ‘‡(ğ‘) = ğ‘‡(ğ‘/2) + ğ‘‚(1)

## Binary Tree Traversal
> ğ‘‡(ğ‘) = 2ğ‘‡(ğ‘/2) + ğ‘‚(1)

## Merge Sort
> ğ‘‡(ğ‘) = 2ğ‘‡(ğ‘/2) + ğ‘‚(ğ‘)

## Recursion Trees
> ğ‘‡(ğ‘) = ğ‘ğ‘‡(ğ‘/ğ‘) + ğ‘“(ğ‘)
â‡’ ğ‘‡(ğ‘)

# Theorem Statement
> ğ‘‡(ğ‘) = ğ‘ğ‘‡(ğ‘/ğ‘) + ğ‘“(ğ‘)

## Three Cases:
1. ğ‘“(ğ‘) âˆˆ ğ‘‚(ğ‘<sup>ğ‘</sup>) where ğ‘ < log<sub>ğ‘</sub>ğ‘
2. ğ‘“(ğ‘) âˆˆ Î˜(ğ‘<sup>ğ‘</sup>log<sup>ğ‘˜</sup>ğ‘) where ğ‘ = log<sub>ğ‘</sub>ğ‘
3. ğ‘“(ğ‘) âˆˆ Î©(ğ‘<sup>ğ‘</sup>) where ğ‘ > log<sub>ğ‘</sub>ğ‘


### Theorem Statement Case 1:
ğ‘‡(ğ‘) = ğ‘ğ‘‡(ğ‘/ğ‘) + ğ‘“(ğ‘)  
- ğ‘“(ğ‘) âˆˆ ğ‘‚(ğ‘<sup>ğ‘</sup>) where ğ‘ < log<sub>ğ‘</sub>ğ‘

#### Result:
> ğ‘‡(ğ‘) âˆˆ Î˜(ğ‘<sup>log<sub>ğ‘</sub>ğ‘</sup>)

#### Example (binary tree traversal)
ğ‘‡(ğ‘) = 2ğ‘‡(ğ‘/2) + 1
- ğ‘ = 2, ğ‘ = 2, log<sub>ğ‘</sub>ğ‘ = 1; ğ‘“(ğ‘) = 1 âˆˆ ğ‘‚(ğ‘<sup>0</sup>)
So
> ğ‘‡(ğ‘) âˆˆ Î˜(ğ‘<sup>1</sup>) = Î˜(ğ‘)

### Theorem Statement Case 2:
ğ‘‡(ğ‘) = ğ‘ğ‘‡(ğ‘/ğ‘) + ğ‘“(ğ‘)
- ğ‘“(ğ‘) âˆˆ Î˜(ğ‘<sup>ğ‘</sup>log<sup>ğ‘˜</sup>ğ‘) where ğ‘ = log<sub>ğ‘</sub>ğ‘

#### Result:
> ğ‘‡(ğ‘) âˆˆ Î˜(ğ‘<sup>log<sub>ğ‘</sub>ğ‘</sup>log<sup>ğ‘˜+1</sup>ğ‘)

#### Example (binary search)
ğ‘‡(ğ‘) = ğ‘‡(ğ‘/2) + 1
- ğ‘ = 1, ğ‘ = 2, log<sub>ğ‘</sub>ğ‘ = 0; ğ‘“(ğ‘) = 1 âˆˆ Î˜(ğ‘<sup>0</sup>)
So
> ğ‘‡(ğ‘) âˆˆ Î˜(ğ‘<sup>0</sup>log<sup>1</sup>ğ‘) = Î˜(logğ‘)

#### Example (merge sort)
ğ‘‡(ğ‘) = 2ğ‘‡(ğ‘/2) + ğ‘
- ğ‘ = 2, ğ‘ = 2, log<sub>ğ‘</sub>ğ‘ = 1; ğ‘“(ğ‘) = ğ‘ âˆˆ Î˜(ğ‘<sup>1</sup>)
So
> ğ‘‡(ğ‘) âˆˆ Î˜(ğ‘<sup>1</sup>log<sup>1</sup>ğ‘) = Î˜(ğ‘logğ‘)

### Theorem Statement Case 3:
ğ‘‡(ğ‘) = ğ‘ğ‘‡(ğ‘/ğ‘) + ğ‘“(ğ‘)
- ğ‘“(ğ‘) âˆˆ Î©(ğ‘<sup>ğ‘</sup>) where ğ‘ > log<sub>ğ‘</sub>ğ‘

#### Result:
> ğ‘‡(ğ‘) âˆˆ Î˜(ğ‘“(ğ‘))

#### Example (quickselect)
ğ‘‡(ğ‘) = ğ‘‡(ğ‘/2) + ğ‘
- ğ‘ = 1, ğ‘ = 2, log<sub>ğ‘</sub>ğ‘ = 0; ğ‘“(ğ‘) = ğ‘ âˆˆ ğ‘‚(ğ‘<sup>1</sup>)
So
> ğ‘‡(ğ‘) âˆˆ Î˜(ğ‘“(ğ‘)) = Î˜(ğ‘)

# Proof
- See CLRS for details:
  - Polynomially smaller/bigger
  - Handling floor âŒŠğ‘¥âŒ‹ and ceiling âŒˆğ‘¥âŒ‰
  - Regularity condition for case 3
